test/Number.v
@@ -3,3 +3,9 @@ From Parsec Require Import
 
 Goal parse (liftA2 pair parseDec parseHex) "23Fa0$" = inr (23, 4000)%N.
 Proof. reflexivity. Qed.
+
+Goal parse parseDec "FFF" = inl (Some "Not a decimal number.").
+Proof. reflexivity. Qed.
+
+Goal parse parseHex "???" = inl (Some "Not a hexadecimal number.").
+Proof. reflexivity. Qed.
