test/Token.v
@@ -15,3 +15,7 @@ Proof. reflexivity. Qed.
 Goal string_of_list_ascii <$>
      parse (manyN 3 (satisfy isdigit)) "412404 Not Found" = inr "412".
 Proof. reflexivity. Qed.
+
+Goal string_of_list_ascii <$>
+     parse (manyN 3 (satisfy isdigit)) "40" = inl None.
+Proof. reflexivity. Qed.
